\begin{proposition}
  \label{proposition:exponential-tightness}
  For each $\stateVar \in \stateSpace$, the family $(\Prb^\epsilon_\stateVar)_{\epsilon>0}$ is exponentially tight on $\pathSpace{[0,\infty)}{\stateSpace}$.
\end{proposition}
\begin{proof}
  \label{proof:proposition:exponential-tightness}
  First note that each family $(\push{\Prb^\epsilon_\stateVar}{\pi_{\underline t}})_{\epsilon>0}$ of finite-dimensional distributions is exponentially tight by Theorem \ref{theorem:fdds}.
  This is because each $\rho > 0$ produces a compact set $K_\rho \defeq \aff^*(\underline t, \cdot, \stateVar)^{-1}[0,\rho] \subseteq \vecSpace^{|\underline t|}$ (by goodness of the rate function) clearly satisfying the following.
  \begin{equation*}
    \limsup_{\epsilon\rightarrow0} \epsilon\log\push{\Prb^\epsilon_\stateVar}{\pi_{\underline t}} (K_\rho^c) \leq -\inf_{\underline\stateVar\in \overline{K_\rho^c}} \aff^*(\underline t, \underline\stateVar, \stateVar) \leq -\rho
  \end{equation*}
  By \cite[Theorem 4.1]{feng2006} (rather, an adaptation of it involving a continuously parameterized family), our desired exponential tightness is obtained if we produce to each $\epsilon, \delta, \lambda, T > 0$ a random variable $\gamma_\epsilon(\delta,\lambda,T)$ with the following dominating property over all $t \in [0,T]$, $s \in [0,\delta]$,
  \begin{gather}
    \label{eq:gamma-dominating}
    \Exp_{\Prb_\stateVar}\Big(
      \exp\big( \epsilon^{-1} \lambda \big( |\Xe_{t+s}-\Xe_t| \wedge 1 \big) 
      | \scrF^\epsilon_t \Big) 
    \leq \Exp_{\Prb_\stateVar}\Big( 
      \exp\gamma_\epsilon(\delta, \lambda, T) 
      | \scrF^\epsilon_t \Big),
  \end{gather}
  such that the following equalities are true for all $\lambda > 0$.
  \begin{gather}
    \label{eq:no-gamma-bound}
    \lim_{\delta\rightarrow0} \limsup_{\epsilon\rightarrow0} 
      \epsilon\log\Exp_{\Prb_\stateVar}\exp\big( 
        \epsilon^{-1}\lambda \big(|\Xe_\delta - \Xe_0| \wedge 1\big) 
      \big) = 0 \\
    \label{eq:gamma-bound}
    \lim_{\delta\rightarrow0} \limsup_{\epsilon\rightarrow0} \epsilon\log\Exp_{\Prb_\stateVar}\exp\gamma_\epsilon(\delta,\lambda, T) = 0 
  \end{gather}
  To show this fact, first note that, by Proposition \ref{proposition:real-moments-revisit}\ref{proposition:real-moments-revisit:aff-uniform-bound}, to each $\lambda > 0$ there exist $\delta_\lambda > 0$ and $C_\lambda > 0$ such that the following inequality holds.
  \begin{equation*}
    \big| \aff(t, \momentVar, \stateVar) - \aff(0, \momentVar, \stateVar) \big| \leq C_\lambda \cdot t \cdot \big( 1 + |\stateVar| \big), \quad t \in [0,\delta_\lambda], ~ \momentVar \in  \closedBall{0}{\lambda\sqrt d}, ~ \stateVar \in  \stateSpace
  \end{equation*}
  We then define the following function $f_\epsilon(\cdot,\delta,\lambda): \stateSpace \rightarrow \bbR$ for each $\epsilon > 0$, $\lambda > 0$, and $\delta \in [0,\delta_\lambda]$.
  \begin{equation*}
    f_\epsilon(\stateVar',\delta,\lambda) \defeq \log 2d + \frac{1}{\epsilon} \cdot C_\lambda \cdot \delta \cdot \big( 1 + |\stateVar| \big)
  \end{equation*}
  We now define $\gamma_\epsilon(\delta, \lambda, T) \defeq f_\epsilon\big( \Xe_t, \delta, \lambda \big)$.

  Note that for all $\lambda, \epsilon, t > 0$, $\delta \in [0,\delta_\lambda]$, and $s \in [0,\delta]$, we use Proposition \ref{proposition:aff-asymptotics} to get the following.
  \begin{align}
    \notag
    &\Exp_{\Prb_\stateVar}\Big(
      \exp\big( \epsilon^{-1} \lambda \big( |\Xe_{t+s}-\Xe_t| \wedge 1 \big) 
      | \scrF^\epsilon_t \Big)  \tag*{} \\
    \notag
    &\leq \Exp_{\Prb_\stateVar}\Big(
      \exp\big( \epsilon^{-1} \lambda \big| \Xe_{t+s}-\Xe_t \big|  \big)
      | \scrF^\epsilon_t \Big) \\
    \notag
    &\leq \sum_{\ell=0}^1 \sum_{i=1}^d \Exp_{\Prb_\stateVar}\bigg(
      \exp\Big( \Bprj{(-1)^\ell\epsilon^{-1}\lambda\sqrt d  \basisVec^i}{\Xe_{t+s}-\Xe_t} \Big)
      | \scrF^\epsilon_t \bigg) \\
    \notag
    &= \sum_{\ell=0}^1 \sum_{i=1}^d \exp\bigg( 
      \epsilon^{-1}\aff\Big(s, (-1)^\ell\lambda\sqrt d \basisVec^i, \Xe_t \Big) 
      - \epsilon^{-1}\Bprj{(-1)^\ell\lambda\sqrt d \basisVec^i}{\Xe_t} \bigg) \\
    \notag
    &\leq 2d \cdot \exp\bigg( \frac1\epsilon \cdot C_\lambda \cdot \delta \cdot \big( 1 + |\Xe_t| \big) \bigg) \\
    &= \exp f_\epsilon(\Xe_t, \delta, \lambda)
    \label{eq:verify-gamma-dominating}
  \end{align}
  Note that (\ref{eq:verify-gamma-dominating}) makes (\ref{eq:gamma-dominating}) true.
  \begin{align*}
    &\Exp_{\Prb_\stateVar}\Big( \exp\big( \epsilon^{-1} \lambda \big( |\Xe_{t+s}-\Xe_t| \wedge 1 \big) | \scrF^\epsilon_t \Big) \\
    &\leq \exp f_\epsilon(\Xe_t, \delta, \lambda) \\
    &= \exp \gamma_\epsilon(\delta, \lambda,T) \\
    &= \Exp_{\Prb_\stateVar}\Big( \exp\gamma_\epsilon(\delta,\lambda,T) | \scrF^\epsilon_t \Big)
  \end{align*}
  For (\ref{eq:no-gamma-bound}), we also use (\ref{eq:verify-gamma-dominating}).
  \begin{align*}
    &\hspace{-1em}\lim_{\delta\rightarrow0} \limsup_{\epsilon\rightarrow0} 
      \epsilon\log\Exp_{\Prb_\stateVar}\exp\big( 
        \epsilon^{-1}\lambda \big(|\Xe_\delta - \Xe_0| \wedge 1\big) 
      \big)  \tag*{} \\
    &=\lim_{\delta\rightarrow0} \limsup_{\epsilon\rightarrow0} 
      \epsilon\log\Exp_{\Prb_\stateVar}
      \Exp_{\Prb_\stateVar}\Big(
      \exp\big(\epsilon^{-1}\lambda \big(|\Xe_\delta - \Xe_0| \wedge 1\big) \big)
      |\scrF^\epsilon_0 \Big) \\
    &\leq \lim_{\delta\rightarrow0}\limsup_{\epsilon\rightarrow0} \epsilon\log\Exp_{\Prb_\stateVar} \exp f_\epsilon(\Xe_0, \delta, \lambda) \\
    &= \lim_{\delta\rightarrow0}\limsup_{\epsilon\rightarrow0} \Big( \epsilon\log 2d + C_\lambda \cdot \delta \cdot \big( 1 + |\stateVar| \big) \Big) \\
    &= 0
  \end{align*}

  Using Proposition \ref{proposition:real-moments-revisit}\ref{proposition:real-moments-revisit:big-time-small-moments}, to each $\lambda > 0$, there exists $\delta_\lambda' > 0$ such that $B(0,\delta_\lambda) \subseteq \momentSpace(\delta_\lambda')$.
  Now, for any $\delta < \delta_\lambda \wedge \delta_\lambda'/(2C_\lambda\sqrt d)$, we again use Proposition \ref{proposition:aff-asymptotics} to get the following.
  \begin{align*}
    &\hspace{-1em}\epsilon\log\Exp_{\Prb_\stateVar}\Big( \exp \gamma_\epsilon(\delta, \lambda,T) \Big) \tag*{} \\
    &=\epsilon\log\Exp_{\Prb_\stateVar}\Big( \exp f_\epsilon(\Xe_t, \delta, \lambda) \Big) \tag*{} \\
    &= \epsilon\log 2d + C_\lambda \cdot\delta + \epsilon\log \Exp_{\Prb_\stateVar}\exp\big(\epsilon^{-1}C_\lambda\delta |\Xe_t| \big) \\
    &\leq \epsilon\log 2d + C_\lambda \cdot\delta + \epsilon\log \sum_{\ell=0}^1\sum_{i=1}^d \Exp_{\Prb_\stateVar}\exp\bprj{(-1)^\ell\epsilon^{-1}C_\lambda \delta\sqrt d \basisVec^i}{\Xe_t} \\
    &\leq 2\epsilon\log2d + C_\lambda \cdot \delta + \max_{\substack{\ell=0,1\\i=1,\ldots,d\\k=1,\ldots,|\underline t|}} \epsilon\log\Exp_{\Prb_\stateVar} \exp\Bprj{ (-1)^\ell \epsilon^{-1} C_\lambda\delta \sqrt d \basisVec^i}{\Xe_t} \\
    &\leq 2\epsilon\log2d + C_\lambda \cdot \delta + \max_{\substack{\ell=0,1\\i=1,\ldots,d\\k=1,\ldots,|\underline t|}} \aff\Big( t, (-1)^\ell C_\lambda \delta\sqrt d \basisVec^i, \stateVar\Big)
  \end{align*}
  This gives us (\ref{eq:gamma-bound}).
\end{proof}
